LeanStlc.lean
@@ -5,5 +5,6 @@ import LeanStlc.Typing
 import LeanStlc.Preservation
 import LeanStlc.Progress
 import LeanStlc.WeakNorm
+import LeanStlc.SNi
 import LeanStlc.StrongNorm
 import LeanStlc.Infer
